---
layout: posts
author: Huan
title: RNN backprop thru time(BPTT part 2) $$\frac{\delta h_{t}} {\delta h_{t-1}}$$
---

Notes on the math for RNN back propagation through time(BPTT), part 2. The 1st
derivative of $$h_t$$ with respect to $$h_{t-1}$$.

---
Given a series:
$$X = \{x_1, x_2...x_n\}$$

Given a set of functions that takes in $$X$$:

$$Y = F(X)$$

We have a vector of functions:

$$Y =
\begin{pmatrix}
f_1(X) \\
f_2(X) \\
. \\
. \\
. \\
f_n(X) \\
\end{pmatrix}$$

---

A Jacobian is a matrix of 1st derivatives of the functions:

$$\begin{pmatrix}
\frac{\delta y_1} {\delta x_1} & \frac{\delta y_1} {\delta x_2} & ... & \frac{\delta y_1} {\delta x_n} \\
. & . & ... & .\\
. & . & ... & .\\
. & . & ... & .\\
\frac{\delta y_n} {\delta x_1} & \frac{\delta y_n} {\delta x_2} & ... & \frac{\delta y_n} {\delta x_n}
\end{pmatrix}$$

For the calculations below, we are only interested in the diagonal derivatives
which are terms with the same subscript in the nominator & denominator (i.e: derivatives with respect to the same time step).

$$\frac{\delta h_t} {\delta E_t} = diag(f'(E_t))$$

---

Deriving $$\frac{\delta h_t} {\delta h_{t-1}}$$:

$$Vx_t + Wh_{t-1} + b_{h} = E_t$$

$$h_{t} = f_{h} (Vx_t + Wh_{t-1} + b_{h}) = f_{h}(E_t)$$

$$\frac{\delta h_t} {\delta E_t} = diag(f'(E_t))$$

$$\frac{\delta E_t} {\delta h_{t-1}} = W$$

$$\frac{\delta h_t} {\delta h_{t-1}} =
\frac{\delta h_t} {\delta E_t}
\frac{\delta E_t} {\delta h_{t-1}} =
diag(f'(E_t)) W$$

---

<br>
